Imp/features/exp_mut.v
@@ -1,28 +1,50 @@
-From Imp Require Export header_extensible.
+From Imp Require Export header_extensible context.
+From Stdlib Require Export Lists.List.
+
 
 Section exp_mut.
     Variable exp : Type.
 
+    Notation loc := nat.
+
     Inductive exp_mut : Type := 
-        | exp_loc : nat -> exp_mut
-        | exp_set : exp -> exp -> exp_mut
+        | exp_loc   : loc -> exp_mut
+        | exp_setref   : exp -> exp -> exp_mut
         | exp_deref : exp -> exp_mut
-        | exp_ref : exp -> exp_mut
+        | exp_ref   : exp -> exp_mut
     .
 
     Context `{Hretr : retract exp_mut exp}.
 
     Definition exp_loc_ (n : nat) : _ := inj (exp_loc n).
-    Definition exp_set_ (e1 e2 : exp) : _ := inj (exp_set e1 e2).
+    Definition exp_setref_ (e1 e2 : exp) : _ := inj (exp_setref e1 e2).
     Definition exp_deref_ (e : exp) : _ := inj (exp_deref e).
     Definition exp_ref_ (e : exp) : _ := inj (exp_ref e).
+
+    Ltac unfold_mut :=
+        match goal with
+        | [ H : context [exp_loc_    ?x] |- _] => unfold exp_loc_ in H
+        | [ H : context [exp_setref_ ?x] |- _] => unfold exp_setref_ in H
+        | [ H : context [exp_deref_  ?x] |- _] => unfold exp_deref_ in H
+        | [ H : context [exp_ref_    ?x] |- _] => unfold exp_ref_ in H
+        | [ |- context [exp_loc_     ?x]] => unfold exp_loc_
+        | [ |- context [exp_setref_  ?x]] => unfold exp_setref_
+        | [ |- context [exp_deref_   ?x]] => unfold exp_deref_
+        | [ |- context [exp_ref_     ?x]] => unfold exp_ref_
+    end.
+
+    Ltac simpl_inj := 
+        repeat unfold_mut; match goal with 
+            | [ H : inj ?x = inj ?y |- _ ] => apply retract_inj in H
+        end
+    .
 
     Variable open_rec : nat -> exp -> exp -> exp.
 
     Definition open_rec_mut (k : nat) (s : exp) (t : exp_mut) : exp := 
         match t with 
             | exp_loc n => inj (exp_loc n)
-            | exp_set v x => inj (exp_set (open_rec k s x) (open_rec k s v))
+            | exp_setref v x => inj (exp_setref (open_rec k s x) (open_rec k s v))
             | exp_deref x => inj (exp_deref (open_rec k s x))
             | exp_ref x => inj (exp_ref (open_rec k s x))
         end
@@ -33,40 +55,102 @@ Section exp_mut.
 
     
     Variable lc' : nat -> exp -> Prop.
-    Variable open_rec_lc :forall s t n, lc' 0 s -> lc' (S n) t -> lc' n (open_rec n s t).
+    Variable open_rec_lc : forall s t n, lc' 0 s -> lc' (S n) t -> lc' n (open_rec n s t).
     Variable lc_weaken   : forall s n m, n <= m  -> lc' n s -> lc' m s.
 
 
     Inductive lc'_mut : nat -> exp -> Prop := 
-        | lc_loc n l: lc'_mut n (exp_loc_ l)
-        | lc_set n v x : lc' n v -> lc' n x -> lc'_mut n (exp_set_ v x)
+        | lc_loc n l   : lc'_mut n (exp_loc_ l)
+        | lc_setref n v x : lc' n v -> lc' n x -> lc'_mut n (exp_setref_ v x)
         | lc_deref n x : lc' n x -> lc'_mut n (exp_deref_ x)
-        | lc_ref n x : lc' n x -> lc'_mut n (exp_ref_ x)
+        | lc_ref n x   : lc' n x -> lc'_mut n (exp_ref_ x)
     .
 
     Variable retract_lc: forall n e, lc'_mut n e -> lc' n e.
     Variable retract_lc_rev: forall n e, lc' n (inj e) -> lc'_mut n (inj e).
 
     Definition lc_weaken_mut : forall s n m, n <= m -> lc'_mut n s -> lc' m s.
-    Proof. Admitted.
+    Proof. 
+        intros s n m le H0. destruct H0; apply retract_lc; constructor; apply lc_weaken with (n := n); easy.
+    Defined.
 
     Definition open_rec_lc_mut : forall s t n, lc' 0 s -> lc'_mut (S n) t -> lc' n (open_rec n s t).
-    Proof. Admitted.
+    Proof.
+        intros s t n lc_s H0. inversion H0; subst;
+        repeat unfold_mut;
+        rewrite retract_open_rec; simpl;
+        apply retract_lc; constructor; try apply open_rec_lc; try easy.
+    Defined.
 
     Variable value : exp -> Prop.
+    Variable value_lc : forall v, value v -> lc' 0 v.
 
     Inductive value_mut : exp -> Prop := 
+        | value_loc l : value_mut (exp_loc_ l)
     .
 
+    Definition value_lc_mut : forall v, value_mut v -> lc' 0 v.
+    Proof.
+        intros. induction H. apply retract_lc. constructor.
+    Defined.
+
     Variable Ctx : Type.
+    Context `{hasProj Ctx (Env (sig value))}.
+
     Variable step : Ctx -> exp -> Ctx -> exp -> Prop.
     Variable preservation : forall c e c' e', lc' 0 e -> step c e c' e' -> lc' 0 e'.
+    
 
-
-    Inductive step_mut : Ctx -> exp -> Ctx -> exp -> Prop :=
+    Inductive step_mut : Ctx -> exp -> Ctx -> exp -> Prop := 
+        (* set *)
+        | step_setref c l v (vp : value v):
+            Env.mem l (get_proj c) = true ->
+            step_mut c 
+                    (exp_setref_ (exp_loc_ l) v) 
+                    (set_proj (Env.add l (exist _ v vp) (get_proj c)) c) 
+                    (exp_loc_ l)
+        | step_setref_red_l s c l c' l': 
+            step c l c' l' -> 
+            step_mut c (exp_setref_ l s) c' (exp_setref_ l' s)
+        | step_setref_red l c s c' s': 
+            step c s c' s' -> 
+            step_mut c (exp_setref_ (exp_loc_ l) s) c' (exp_setref_ (exp_loc_ l) s')
+        (* dereference *)
+        | step_deref c l sig_v: 
+            Env.find l (get_proj c) = Some sig_v -> 
+            step_mut c (exp_deref_ (exp_loc_ l)) c (proj1_sig sig_v) 
+        | step_deref_red c s c' s': 
+            step c s c' s' -> step_mut c (exp_deref_ s) c (exp_deref_ s')
+        (* reference *)
+        | step_ref c v c' l : 
+            Env.mem l (get_proj c) = false ->
+            step_mut c (exp_ref_ v) c' (exp_loc_ l)
+        | step_ref_red c s c' s': 
+            step c s c' s' -> step_mut c (exp_ref_ s) c' (exp_ref_ s')
     .
 
     Definition preservation_mut : forall c e c' e', lc' 0 e -> step_mut c e c' e' -> lc' 0 e'.
-    Proof. Admitted.
+    Proof.
+        intros c e c' e' lc_e.
+        induction 1. 
+        - apply retract_lc. constructor.
+        - apply retract_lc_rev in lc_e. inversion lc_e; subst; try simpl_inj; try easy.
+          apply retract_lc. constructor.
+            + inversion H1. subst. apply (preservation _ _ _ _ H2 H0).
+            + inversion H1. subst. easy.
+        - apply retract_lc_rev in lc_e. inversion lc_e; subst; try simpl_inj; try easy.
+          apply retract_lc. constructor.
+            + apply retract_lc. constructor.
+            + inversion H1. subst. apply (preservation _ _ _ _ H4 H0).
+        - destruct sig_v. simpl. 
+          apply value_lc. easy.
+        - apply retract_lc_rev in lc_e. inversion lc_e; subst; try simpl_inj; try easy.
+          inversion H1. subst. apply retract_lc. constructor. apply (preservation _ _ _ _ H3 H0).
+        - unfold exp_loc_. apply retract_lc. constructor.
+        - unfold exp_ref_. apply retract_lc. constructor. 
+          apply retract_lc_rev in lc_e. inversion lc_e; subst; try simpl_inj; try easy.
+          inversion H1. subst.
+          apply (preservation c s c' s'); easy.
+    Defined.
 
 End exp_mut.
